open-vm: add beginning of specification for branch_eq

Garden/OpenVM/BranchEq/core_with_monad.v
@@ -1,6 +1,21 @@
 Require Import Garden.Plonky3.MLessEffects.
 
 (*
+pub struct ImmInstruction<T> {
+    pub is_valid: T,
+    pub opcode: T,
+    pub immediate: T,
+}
+*)
+Module ImmInstruction.
+  Record t : Set := {
+    is_valid : Z;
+    opcode : Z;
+    immediate : Z;
+  }.
+End ImmInstruction.
+
+(*
 pub struct AdapterAirContext<T, I: VmAdapterInterface<T>> {
   pub to_pc: Option<T>,
   pub reads: I::Reads,
@@ -10,12 +25,16 @@ pub struct AdapterAirContext<T, I: VmAdapterInterface<T>> {
 *)
 (* TODO: move it to another file, as this is actually related to `integration_api.rs` *)
 Module AdapterAirContext.
-  Record t : Set := {
+  Record t {NUM_LIMBS : Z}: Set := {
     to_pc : option Z;
-    (* reads : I::Reads;
-    writes : I::Writes;
-    instruction : I::ProcessedInstruction; *)
+    (* I::Reads: From<[[AB::Expr; NUM_LIMBS]; 2]>, *)
+    reads : Array.t Z NUM_LIMBS * Array.t Z NUM_LIMBS;
+    (* I::Writes: Default, *)
+    writes : unit;
+    (* I::ProcessedInstruction: From<ImmInstruction<AB::Expr>>, *)
+    instruction : ImmInstruction.t;
   }.
+  Arguments t : clear implicits.
 End AdapterAirContext.
 
 (* TODO: from `instructions.rs`, move there *)
@@ -65,18 +84,17 @@ pub struct BranchEqualCoreAir<const NUM_LIMBS: usize> {
 }
 *)
 Module BranchEqualCoreAir.
-  Record t {NUM_LIMBS : Z} : Set := {
+  Record t : Set := {
     offset : Z;
     pc_step : Z;
   }.
-  Arguments t : clear implicits.
 End BranchEqualCoreAir.
 
 Definition eval {p} `{Prime p} {NUM_LIMBS : Z}
-    (self : BranchEqualCoreAir.t NUM_LIMBS)
+    (self : BranchEqualCoreAir.t)
     (local : BranchEqualCoreCols.t NUM_LIMBS)
     (from_pc : Z) :
-    M.t AdapterAirContext.t :=
+    M.t (AdapterAirContext.t NUM_LIMBS) :=
   let flags : list Z := [
     local.(BranchEqualCoreCols.opcode_beq_flag);
     local.(BranchEqualCoreCols.opcode_bne_flag)
@@ -97,20 +115,20 @@ Definition eval {p} `{Prime p} {NUM_LIMBS : Z}
   let b : Array.t Z NUM_LIMBS := local.(BranchEqualCoreCols.b) in
   let inv_marker : Array.t Z NUM_LIMBS := local.(BranchEqualCoreCols.diff_inv_marker) in
 
-  let cmp_eq : Z :=
-    BinOp.add
-      (BinOp.mul local.(BranchEqualCoreCols.cmp_result) local.(BranchEqualCoreCols.opcode_beq_flag))
-      (BinOp.mul (MLessEffects.not local.(BranchEqualCoreCols.cmp_result)) local.(BranchEqualCoreCols.opcode_bne_flag))
-    in
+  let* cmp_eq : Z :=
+    M.pure (
+      BinOp.add
+        (BinOp.mul local.(BranchEqualCoreCols.cmp_result) local.(BranchEqualCoreCols.opcode_beq_flag))
+        (BinOp.mul (MLessEffects.not local.(BranchEqualCoreCols.cmp_result)) local.(BranchEqualCoreCols.opcode_bne_flag))
+    ) in
 
-  let* sum : Z :=
-    List.fold_left
-      (fun acc i =>
-        let i := Z.of_nat i in
-        let* _ := assert_zero (BinOp.mul cmp_eq (BinOp.sub (Array.get a i) (Array.get b i))) in
-        M.pure (BinOp.add acc (BinOp.mul (Array.get inv_marker i) (BinOp.sub (Array.get a i) (Array.get b i))))
-      )
-      Z.zero (List.seq 0 (Z.to_nat NUM_LIMBS)) in
+  let* _ := M.for_in_zero_to_n NUM_LIMBS (fun i =>
+    assert_zero (BinOp.mul cmp_eq (BinOp.sub (Array.get a i) (Array.get b i)))
+  ) in
+  let* sum : Z := M.sum_for_in_zero_to_n NUM_LIMBS (fun i =>
+    BinOp.mul (Array.get inv_marker i) (BinOp.sub (Array.get a i) (Array.get b i))
+  ) in
+  let sum := BinOp.add sum cmp_eq in
   let* _ := when is_valid (assert_one sum) in
 
   let flags_with_opcode_integer : list (Z * Z) :=
@@ -139,4 +157,264 @@ Definition eval {p} `{Prime p} {NUM_LIMBS : Z}
 
   M.pure {|
     AdapterAirContext.to_pc := Some to_pc;
+    AdapterAirContext.reads := (a, b);
+    AdapterAirContext.writes := tt;
+    AdapterAirContext.instruction := {|
+      ImmInstruction.is_valid := is_valid;
+      ImmInstruction.opcode := expected_opcode;
+      ImmInstruction.immediate := local.(BranchEqualCoreCols.imm);
+    |};
   |}.
+
+Module Array.
+  Parameter to_limbs : forall (NUM_LIMBS value : Z), Array.t Z NUM_LIMBS.
+End Array.
+
+Module Input.
+  Record t : Set := {
+    a : Z;
+    b : Z;
+    opcode : BranchEqualOpcode.t;
+    imm : Z;
+    to_pc : Z;
+  }.
+
+  Module Extra.
+    Record t : Set := {
+      cmp_result : Z;
+      diff_inv_marker : Z;
+    }.
+  End Extra.
+
+  Definition to_cols {NUM_LIMBS : Z} (input : t) (extra : Extra.t) :
+    BranchEqualCoreCols.t NUM_LIMBS :=
+  {|
+    BranchEqualCoreCols.a := Array.to_limbs NUM_LIMBS input.(a);
+    BranchEqualCoreCols.b := Array.to_limbs NUM_LIMBS input.(b);
+    BranchEqualCoreCols.cmp_result := extra.(Extra.cmp_result);
+    BranchEqualCoreCols.imm := input.(imm);
+    BranchEqualCoreCols.opcode_beq_flag :=
+      match input.(opcode) with
+      | BranchEqualOpcode.BEQ => 1
+      | BranchEqualOpcode.BNE => 0
+      end;
+    BranchEqualCoreCols.opcode_bne_flag :=
+      match input.(opcode) with
+      | BranchEqualOpcode.BEQ => 0
+      | BranchEqualOpcode.BNE => 1
+      end;
+    BranchEqualCoreCols.diff_inv_marker :=
+      Array.to_limbs NUM_LIMBS extra.(Extra.diff_inv_marker);
+  |}.
+End Input.
+
+Module Output.
+  Record t : Set := {
+    to_pc : Z;
+    reads : Z * Z;
+    writes : unit;
+    instruction : ImmInstruction.t;
+  }.
+
+  Definition to_adapter_air_context {NUM_LIMBS : Z} (output : t) :
+    AdapterAirContext.t NUM_LIMBS :=
+  {|
+    AdapterAirContext.to_pc := Some output.(to_pc);
+    AdapterAirContext.reads :=
+      let '(a, b) := output.(reads) in
+      (Array.to_limbs NUM_LIMBS a, Array.to_limbs NUM_LIMBS b);
+    AdapterAirContext.writes := output.(writes);
+    AdapterAirContext.instruction := output.(instruction);
+  |}.
+
+  (**
+    - If opcode_beq_flag is true and a is equal to b, then to_pc == pc + imm, otherwise to_pc == pc + 4
+    - If opcode_bne_flag is true and a is not equal to b, then to_pc == pc + imm, otherwise to_pc == pc + 4
+  *)
+  Definition of_input (core_air : BranchEqualCoreAir.t) (input : Input.t) : t := {|
+    to_pc :=
+      match input.(Input.opcode) with
+      | BranchEqualOpcode.BEQ =>
+        if input.(Input.a) =? input.(Input.b) then
+          input.(Input.to_pc) + input.(Input.imm)
+        else
+        input.(Input.to_pc) + core_air.(BranchEqualCoreAir.pc_step)
+      | BranchEqualOpcode.BNE =>
+        if negb (input.(Input.a) =? input.(Input.b)) then
+          input.(Input.to_pc) + input.(Input.imm)
+        else
+          input.(Input.to_pc) + 4
+      end;
+    reads := (input.(Input.a), input.(Input.b));
+    writes := tt;
+    instruction := {|
+      ImmInstruction.is_valid := 1;
+      ImmInstruction.opcode :=
+        core_air.(BranchEqualCoreAir.offset) + match input.(Input.opcode) with
+        | BranchEqualOpcode.BEQ => 0
+        | BranchEqualOpcode.BNE => 1
+        end;
+      ImmInstruction.immediate := input.(Input.imm);
+    |};
+  |}.
+End Output.
+
+Smpl Create run_auto.
+
+Axiom assert_bool_zero :
+  {{ M.AssertBool 0 🔽 tt, True }}.
+Smpl Add apply assert_bool_zero : run_auto.
+
+Axiom assert_bool_one :
+  {{ M.AssertBool 1 🔽 tt, True }}.
+Smpl Add apply assert_bool_one : run_auto.
+
+
+Lemma eval_is_valid `{Prime 23} {NUM_LIMBS : Z}
+    (core_air : BranchEqualCoreAir.t)
+    (input : Input.t)
+    (extra : Input.Extra.t)
+    (from_pc : Z) :
+  let cols : BranchEqualCoreCols.t NUM_LIMBS := Input.to_cols input extra in
+  let output : AdapterAirContext.t NUM_LIMBS :=
+    Output.to_adapter_air_context (Output.of_input core_air input) in
+  {{ eval core_air cols from_pc 🔽 output, True }}.
+Proof.
+  cbn.
+  eapply Run.Implies. {
+    unfold eval; cbn.
+    eapply Run.Let with (value := 1) (P1 := True). {
+      destruct input.(Input.opcode); cbn.
+      { eapply Run.Implies. {
+          repeat (
+            (eapply Run.Let; [|intro]) ||
+            smpl run_auto ||
+            apply Run.Pure
+          ).
+        }
+        tauto.
+      }
+      { eapply Run.Implies. {
+          repeat (
+            (eapply Run.Let; [|intro]) ||
+            smpl run_auto ||
+            apply Run.Pure
+          ).
+        }
+        tauto.
+      }
+    }
+    intros [].
+    eapply Run.Let. {
+      smpl run_auto.
+    }
+    intros [].
+    eapply Run.Let. {
+      apply Run.AssertBool.
+    }
+    intros [cmp_result H_cmp_result_eq].
+    rewrite H_cmp_result_eq.
+    set (cmp_eq :=
+      match input.(Input.opcode) with
+      | BranchEqualOpcode.BEQ => cmp_result
+      | BranchEqualOpcode.BNE => negb cmp_result
+      end
+    ).
+    (* match goal with
+    | |- context[M.pure ?e] =>
+      set (cmp_eq := e)
+    end. *)
+    eapply Run.Let with (value := Z.b2z cmp_eq). {
+      destruct input.(Input.opcode), cmp_result; apply Run.Pure.
+    }
+    intros [].
+    eapply Run.Implies. {
+    eapply Run.Let with
+      (P1 :=
+        if cmp_eq then
+          forall i, 0 <= i < NUM_LIMBS ->
+          (Array.to_limbs NUM_LIMBS input.(Input.a)).(Array.get) i =
+          (Array.to_limbs NUM_LIMBS input.(Input.b)).(Array.get) i
+        else
+          True
+      ). {
+      destruct cmp_eq; cbn.
+      { apply Run.ForInZeroToN; intros.
+        unfold assert_zero.
+Admitted.
+(*
+        apply Run.Equal.
+        eapply Run.Let. {
+          smpl run_auto.
+        }
+      }
+      { admit. }
+    }
+
+    eapply Run.Implies. {
+    eapply Run.Let with
+        (value := if cmp_eq then 1 else 0)
+        (P1 :=
+          if cmp_eq then
+            forall (i : nat),
+              (0 <= i < NUM_LIMBS)%nat ->
+              (Array.to_limbs (Z.of_nat NUM_LIMBS) input.(Input.a)).(Array.get) (Z.of_nat i) =
+              (Array.to_limbs (Z.of_nat NUM_LIMBS) input.(Input.b)).(Array.get) (Z.of_nat i)
+          else
+            False
+        ). {
+      destruct cmp_eq; cbn.
+      { rewrite Nat2Z.id.
+        induction NUM_LIMBS; cbn.
+        { admit. }
+        { eapply Run.Implies. {
+          eapply Run.Let. {
+            apply IHNUM_LIMBS.
+        }
+      admit. }
+      { admit. }
+    }
+    intros [].
+    eapply Run.Let. {
+      smpl run_auto.
+    }
+    intros [].
+    eapply Run.Let. {
+      smpl run_auto.
+    }
+    intros [].
+    eapply Run.Let. {
+        { repeat (
+            eapply Run.Let ||
+            eapply Run.AssertBool ||
+            apply Run.Pure
+          ).
+          unfold BinOp.add, BinOp.mul; cbn.
+          assert (H_1_eq : 1 mod p = 1) by admit.
+          repeat (rewrite H_1_eq; cbn).
+          apply Run.Pure.
+        }
+        reflexivity.
+        eapply Run.Replace; [apply Run.Pure |].
+        unfold BinOp.add, BinOp.mul.
+        cbn.
+        assert (H_1_eq : 1 mod p = 1) by admit.
+        repeat (rewrite H_1_eq; cbn).
+        reflexivity.
+      }
+      { repeat (
+          eapply Run.Let ||
+          eapply Run.Equal ||
+          apply Run.Pure
+        ).
+        eapply Run.Replace; [apply Run.Pure |].
+        unfold BinOp.add, BinOp.mul.
+        cbn.
+        assert (H_1_eq : 1 mod p = 1) by admit.
+        repeat (rewrite H_1_eq; cbn).
+        reflexivity.
+      }
+      unfold assert_bool.
+  }
+Qed.
+*)
